backends/riscv/AvgRiscv.lean
@@ -1,2 +1,3 @@
 import AvgRiscv.Impl
 import AvgRiscv.Proofs
+import AvgRiscv.Encode
